fairneris/examples/retransmit_example.v
@@ -1,4 +1,5 @@
 From stdpp Require Import list fin_maps.
+From iris.algebra Require Import excl_auth.
 From iris.proofmode Require Import proofmode.
 From iris.base_logic.lib Require Import invariants.
 From trillium.program_logic Require Import ectx_lifting.
@@ -18,65 +19,76 @@ Definition Aprog (saA saB : socket_address) : expr :=
   let: "f" := (rec: "go" <> := SendTo "shA" #"Hello" #saB;; "go" #()) in
   "f" #().
 
-Definition Bprog shB : expr := ReceiveFrom #(LitSocket shB).
+Definition wait_receive : val :=
+  (λ: "sh",
+    SetReceiveTimeout "sh" #1 #1 ;;
+    let: "go" := rec: "go" <> :=
+     let: "r" := ReceiveFrom "sh" in
+     if: "r" = NONEV then "go" #() else #()%V
+    in "go" #()
+  ).
+(* Definition wait_receive := wait_receive_def. *)
+(* Lemma wait_receive_eq : wait_receive = wait_receive_def. *)
+(* Proof. done. Qed. *)
+(* Opaque wait_receive. *)
 
-Tactic Notation "mu_fuel" :=
-  let solve_fuel _ :=
-    let fs := match goal with |- _ = Some (_, has_fuels _ ?fs) => fs end in
-    iAssumptionCore || fail "wp_pure: cannot find" fs in
-  iStartProof;
-  lazymatch goal with
-  | |- envs_entails _ (MU ?E ?locale None ?P) =>
-      eapply (tac_mu_fuel _ locale E);
-      [let fs := match goal with |- _ = Some (_, has_fuels _ ?fs) => fs end in
-       iAssumptionCore || fail "mu_fuel: cannot find" fs
-      | try apply map_non_empty_singleton; try apply insert_non_empty; try done
-      | try solve_fuel_positive
-      | pm_reduce; simpl_has_fuels; wp_finish
-      ]
-  | _ => fail "wp_pure: not a 'wp'"
-  end.
+Definition Bprog saA saB : expr :=
+  let: "shB" := NewSocket #() in
+  SocketBind "shB" #saB;;
+  wait_receive "shB" ;;
+  SendTo "shB" #"Done" #saA.
 
-Tactic Notation "wp_pure" open_constr(efoc) :=
-  iStartProof;
-  lazymatch goal with
-  | |- envs_entails _ (wp ?s ?E ?locale ?e ?Q) =>
-    let e := eval simpl in e in
-    reshape_expr e ltac:(fun K e' =>
-      idtac K;
-      unify e' efoc;
-      eapply (tac_wp_pure _ _ _ _ _ (@fill base_ectxi_lang K e') _ _ 1); idtac "Hi";
-      [ let fs := match goal with |- _ = Some (_, has_fuels _ ?fs) => fs end in
-       iAssumptionCore || fail "wp_pure: cannot find" fs
-      | tc_solve
-      | try solve_fuel_positive
-      | try apply map_non_empty_singleton; try apply insert_non_empty; try done
-      | try naive_solver
-      | tc_solve
-      | pm_reduce; simpl_has_fuels; wp_finish
-      ])
-      (* [try tc_solve                       (* PureExec *) *)
-      (* |try solve_vals_compare_safe    (* The pure condition for PureExec *) *)
-      (* |try tc_solve                       (* IntoLaters *) *)
-      (* |try wp_finish                      (* new goal *) *)
-      (* ]) *)
-    || fail "wp_pure: cannot find" efoc "in" e "or" efoc "is not a redex"
-  end.
+Canonical Structure retransmitO := leibnizO retransmit_state.
+
+Class retransmitG Σ := RetransmitG {
+  retransmit_name: gname;
+  retransmit_done_G :> inG Σ (excl_authR retransmitO);
+ }.
+Class retransmitPreG Σ := {
+  retransmit_done_PreG :> inG Σ (excl_authR retransmitO);
+ }.
+Definition retransmitΣ : gFunctors :=
+  #[ anerisΣ (live_model_of_user retransmit_model);
+     GFunctor (excl_authR retransmitO) ].
+
+Global Instance subG_retransmitΣ {Σ} : subG retransmitΣ Σ → retransmitPreG Σ.
+Proof. solve_inG. Qed.
 
 Section with_Σ.
   Context `{anerisG _ _ (live_model_of_user retransmit_model) Σ}.
+  Context `{!retransmitG Σ}.
   Let Ns := nroot .@ "retransmit".
 
-  Notation loA := (ip_of_address saA, tidA).
+  Definition ipA := "0.0.0.0".
+  Definition saA := SocketAddressInet ipA 80.
 
-  Definition retinv : iProp Σ := ∃ st, frag_model_is st ∗ True.
+  Definition ipB := "0.0.0.1".
+  Definition saB := SocketAddressInet ipB 80.
 
-  Lemma wp_A f (Hf: f > 9) :
-    {{{ inv Ns retinv ∗ frag_free_roles_are ∅ ∗ is_node loA.1 ∗ saB ⤇ (λ _, True) ∗
-          loA ↦M {[ Arole := f ]} ∗ saA ⤳ (∅, ∅) ∗
+  Definition mAB := mkMessage saA saB "Hello".
+
+  Definition retinv : iProp Σ := ∃ st, frag_model_is st ∗ own retransmit_name (●E st).
+
+  Lemma token_update γ (st st' st'' : retransmit_state) :
+    own γ (●E st) ∗ own γ (◯E st'') ==∗ own γ (●E st') ∗ own γ (◯E st').
+  Proof.
+    rewrite -!own_op. iApply own_update. apply excl_auth_update.
+  Qed.
+
+  Lemma token_agree γ (st st' : retransmit_state) :
+    own γ (●E st) -∗ own γ (◯E st') -∗ ⌜ st = st' ⌝.
+  Proof.
+    iIntros "HA HB". iCombine "HB HA" as "H".
+    iDestruct (own_valid with "H") as "%Hval".
+    iPureIntro. by apply excl_auth_agree_L.
+  Qed.
+
+  Lemma wp_A tid f (Hf: f > 9) :
+    {{{ inv Ns retinv ∗ frag_free_roles_are ∅ ∗ is_node ipA ∗ saB ⤇ (λ _, True) ∗
+          (ipA, tid) ↦M {[ Arole := f ]} ∗ saA ⤳ (∅, ∅) ∗
           free_ports (ip_of_address saA) {[port_of_address saA]} }}}
-      (mkExpr (ip_of_address saA) (Aprog saA saB)) @ loA; ⊤
-    {{{ v, RET v; loA ↦M ∅ }}}.
+      (mkExpr (ip_of_address saA) (Aprog saA saB)) @ (ipA, tid); ⊤
+    {{{ v, RET v; (ipA, tid) ↦M ∅ }}}.
   Proof.
     iIntros (Φ) "(#Hinv & Hfr & #Hisn & #Hmsg & HA & Hrt & Hfp) HΦ".
 
@@ -89,11 +101,9 @@ Section with_Σ.
     mu_fuel.
     iApply wp_value'.
 
-    idtac "ASDLKFJ".
     do 2 wp_pure _.
 
     wp_bind (SocketBind _ _).
-    change "0.0.0.0" with (ip_of_address saA).
     iApply sswp_MU_wp.
     iApply (wp_socketbind with "[Hfp] [Hsh']")=>//=; first done.
     iIntros "Hsh".
@@ -104,7 +114,7 @@ Section with_Σ.
     iAssert (∃ R T, saA ⤳ (R, T) ∗
             [∗ set] m ∈ R, socket_address_group_own {[m_sender m]})%I
       with "[Hrt]" as (R T) "[HRT HR]"; [by eauto|].
-    iAssert (∃ f, ⌜ f > 0 ⌝ ∗ ("0.0.0.0", tidA) ↦M <[Arole:=f]> ∅)%I
+    iAssert (∃ f, ⌜ f > 0 ⌝ ∗ ("0.0.0.0", tid) ↦M <[Arole:=f]> ∅)%I
       with "[HA]" as (f') "[Hf HA]".
     { iExists _. iSplit; last iFrame. iPureIntro. lia. }
 
@@ -120,7 +130,7 @@ Section with_Σ.
     iModIntro.
 
     iApply (wp_send _ _ false with "[Hsh] [HRT] [Hmsg]")=>//=>//=>//.
-    iIntros "Hsh HRT".
+    iNext. iIntros "Hsh HRT".
 
     iApply (mu_step_model _ _ _ _ ∅ ∅ _ st with "Hst [HA] [Hfr //]").
     { constructor. }
@@ -129,130 +139,191 @@ Section with_Σ.
     { rewrite fmap_empty map_union_empty //. }
     iIntros "Hst HA Hfr".
 
-    iMod ("Hclose" with "[Hst]").
-    { iNext. iExists st. naive_solver. }
+    iMod ("Hclose" with "[Hst Hrest]").
+    { iNext. iExists st. iFrame. }
     iModIntro.
     simpl.
     rewrite /= ?map_union_empty //.
 
     iApply wp_value'.
     do 2 wp_pure _.
-    iApply ("IH" $! 8 with "[$] [$] [$] [$] [$] [$] []").
+    iApply ("IH" with "[$] [$] [$] [$] [$] [$] []").
     iPureIntro; lia.
   Qed.
 
-  Lemma wp_B s E shB :
-    {{{ shB ↪[ip_of_address saB] sB ∗ saB ⤳ (∅,∅) ∗ saB ⤇ (λ _, True) ∗
-        live_role_frag_own Brole }}}
-      (mkExpr (ip_of_address saB) (Bprog shB)) @ s; (ip_of_address saB, tidB); E
-    {{{ v, RET v; dead_role_frag_own Brole }}}.
+  Lemma wp_wait tid f (Hf: f > 9) sh b R1 T1:
+    {{{ inv Ns retinv ∗ own retransmit_name (◯E retransmit_model.Start) ∗
+          frag_free_roles_are ∅ ∗ is_node ipB ∗ saB ⤇ (λ _, True) ∗
+          (ipB, tid) ↦M {[ Brole := f ]} ∗ saB ⤳ (R1, T1) ∗
+          sh ↪[ipB] {| saddress := Some saB; sblock := b |} }}}
+      (mkExpr (ip_of_address saB) (wait_receive #(LitSocket sh))) @ (ipB, tid); ⊤
+    {{{ v, RET v; ⌜ v.(val_n) = ipB ⌝ ∗ ∃ f' R2 T2, (ipB, tid) ↦M {[ Brole := f' ]} ∗ ⌜ f' > 8 ⌝ ∗
+        own retransmit_name (◯E retransmit_model.Received) ∗
+        saB ⤳ (R2, T2) ∗ sh ↪[ipB] {| saddress := Some saB; sblock := false |}
+    }}}.
   Proof.
-    iIntros (Φ) "(Hsh & Hrt & #HΨ & HB) HΦ".
-    iLöb as "IH".
-    iApply wp_lift_head_step; auto.
-    iIntros (ex atr K tp1 tp2 σ Hexvalid Hex) "(%Hvalid & Hσ & [Hlive_auth Hdead_auth] & Hauth) /=".
-    iMod (steps_auth_update_S with "Hauth") as "Hauth".
-    rewrite (last_eq_trace_ends_in _ _ Hex).
-    iDestruct (aneris_state_interp_network_sockets_coh_valid with "Hσ") as %Hcoh.
-    iDestruct (aneris_state_interp_socket_valid with "Hσ Hsh")
-      as (Sn r) "[%HSn (%Hr & %Hreset)]".
-    iDestruct (live_role_auth_elem_of with "Hlive_auth HB") as %Hrole.
-    destruct (trace_last atr) as [[[] ms] bs] eqn:Heqn; last first.
-    { rewrite Heqn in Hrole. set_solver. }
-    simpl in *.
-    destruct Hvalid as (Hsteps & Hmatch & Hlive & [Hms Hskts]).
-    rewrite Hex in Hskts. rewrite Heqn in Hskts.
-    simpl in *.
-    subst.
-    assert (bs !!! saB = r) as Hbs.
-    { by eapply Hskts. }
-    destruct (decide (r = [])) as [-> | Hneq].
-    - iMod (fupd_mask_intro_subseteq _ ∅ True%I with "[]") as "Hmk";
-        first set_solver; auto.
-      iModIntro. iSplitR.
-      { by iPureIntro; do 4 eexists; eapply SocketStepS; eauto; econstructor. }
-      iIntros (v2' ? ? ? Hstep).
-      inv_head_step.
-      { assert (length (r ++ [m]) = length ([] : list message))
-          as Hdone; [by f_equal|].
-        rewrite app_length /= in Hdone. lia. }
-      rewrite (insert_id (state_sockets σ)); last done.
-      iNext.
-      iMod "Hmk" as "_".
+    iIntros (Φ) "(#Hinv & Htok & #Hfr & Hin & #HsockB & HB & Hrt & Hsh) HΦ".
+    rewrite /wait_receive.
+    wp_pure _.
+
+    wp_bind (SetReceiveTimeout _ _ _).
+
+    iApply sswp_MU_wp.
+    iApply (wp_rcvtimeo_ublock NotStuck ⊤ (ipB, tid) sh _ saB 1 1 with "[Hsh]").
+    3: { auto. }
+    { done. }
+    { lia. }
+    iIntros "Hsh".
+    mu_fuel.
+    iApply wp_value'.
+    do 5 wp_pure _.
+
+    iAssert (∃ f, ⌜ f > 2 ⌝ ∗ (ipB, tid) ↦M <[Brole:=f]> ∅)%I
+      with "[HB]" as (f') "[Hf HB]".
+    { iExists _. iSplit; last iFrame. iPureIntro. lia. }
+
+    clear f Hf.
+    iLöb as "IH" forall (f' R1 T1) "Hf".
+    iDestruct "Hf" as %Hf.
+
+    wp_pure _.
+    wp_bind (ReceiveFrom _).
+
+    iApply sswp_MU_wp_fupd.
+
+    iInv Ns as (st) "(Hst & Hrest)" "Hclose".
+    iModIntro.
+
+    iApply (wp_recv with "[Hsh] [Hrt] [HsockB]")=>//=>//=>//.
+    iNext.
+
+    iDestruct (token_agree with "Hrest Htok") as %->.
+
+    iIntros (om r) "H".
+    iDestruct "H" as "[(%Hr&%Hom&Hsh&Hrt)|(%msg & %Hr & %Hom & %Hdest & Hsh & Hrt & %Hin')]".
+    - simplify_eq.
+      iApply (mu_step_model _ _ _ _ ∅ ∅ _ (retransmit_model.Start : retransmit_model) with "Hst [HB] [Hfr //]").
+      { constructor. }
+      { set_solver. }
+      { set_solver. }
+      { rewrite fmap_empty map_union_empty //. }
+      iIntros "Hst HB Hfr'".
+
+      iMod ("Hclose" with "[Hst Hrest]").
+      { iNext. iExists _. iFrame. }
       iModIntro.
-      iExists (retransmit_model.Start, ms, bs), (inl (Brole, None)).
-      rewrite -message_history_evolution_id.
-      rewrite Heqn.
-      iFrame.
-      iSplitR; last first.
-      { iSplitL; [|done]. by iApply ("IH" with "Hsh Hrt HB HΦ"). }
-      iPureIntro.
-      rewrite /trace_ends_in in Hex.
-      rewrite /trace_ends_in in Hex.
-      split; [econstructor;[done|by econstructor|done]|].
-      rewrite Hex in Hms. rewrite Heqn in Hms.
-      split; [done|].
-      split; [|done].
-      intros ℓ ζ Hlabels Henabled.
-      rewrite right_id_L.
-      rewrite Hex in Hlive. eapply Hlive; [done|by rewrite Heqn].
-    - iMod (fupd_mask_intro_subseteq _ ∅ True%I with "[]") as "Hmk";
-        first set_solver; auto.
-      iModIntro. iSplitR.
-      { iPureIntro. apply last_is_Some in Hneq as [m Hneq].
-        apply last_Some in Hneq as [? ->].
-        do 4 eexists; eapply SocketStepS; eauto; econstructor; eauto 2. }
-      iIntros (v2' ? ? ? Hstep).
-      inv_head_step.
-      iNext.
-      iMod "Hmk" as "_".
-      iAssert (socket_address_group_own {[saB]})%I as "#HsaB".
-      { iDestruct "Hrt" as "[(%send & %recv & _ & _ & _ & $ & _) _]". }
-      rewrite -H1 in Hr.
-      iPoseProof (aneris_state_interp_receive_some saB {[saB]} _ _ _ _ (Some _)
-                   with "[] [$HΨ] [$Hσ] [$Hsh] [Hrt]")
-        as (R' sagT) "(%HinT & #HownT & %Hhist & %HR & Hrt & Hrest)";
-        [by set_solver..| | |].
-      { iFrame "#". iPureIntro. set_solver. }
-      { iDestruct "Hrt" as "[$ Hrt]". }
-      iMod "Hrest" as "(Hσ & Hsh & Ha)".
-      iMod (live_roles_auth_delete with "Hlive_auth HB") as "Hlive_auth".
-      iMod (dead_role_auth_extend _ (Brole : fmrole retransmit_fair_model) with "Hdead_auth")
-        as "[Hdead_auth Hdead_own]"; [by set_solver|].
+      iApply wp_value'.
+      simpl.
+      rewrite !map_union_empty //.
+      do 4 wp_pure _.
+      iApply ("IH" with "[$] [$] [$] [$] [$] [$]").
+      { iPureIntro; lia. }
+    - simplify_eq.
+      iApply (mu_step_model _ _ _ _ ∅ ∅ _ (Received : retransmit_model) with "Hst [HB] [Hfr //]").
+      { constructor. }
+      { set_solver. }
+      { set_solver. }
+      { rewrite fmap_empty map_union_empty //. }
+      iIntros "Hst HB Hfr'".
+
+      iMod (token_update with "[$]") as "[Hrest Htok]".
+      iMod ("Hclose" with "[Hst Hrest]").
+      { iNext. iExists Received. iFrame. }
       iModIntro.
-      iExists (retransmit_model.Received, ms, <[saB:=r]>bs),
-                (inl (Brole, None)).
-      rewrite Heqn Hhist=> /=.
-      rewrite /thread_live_roles_interp /retransmit_live_roles. simpl in *.
-      replace ({[Arole; Brole]} ∖ {[Brole]}) with ({[Arole]} : gset _)
-                                                  by set_solver.
-      replace({[Brole]} ∪ all_roles ∖ {[Arole; Brole]}) with
-        (all_roles ∖ {[Arole]} : gset _) by set_solver.
-      rewrite !right_id_L.
-      iFrame "Hauth Hlive_auth Hdead_auth Hσ".
-      iSplitR "HΦ Hdead_own"; last first.
-      { iSplit; [|done]. iApply wp_value. by iApply "HΦ". }
-      iPureIntro.
-      split; [econstructor;[done|by econstructor|done]|].
-      rewrite Hex in Hms. rewrite Heqn in Hms.
-      split; [done|].
-      split; last first.
-      { split; [done|]. by eapply state_buffers_delete. }
-      intros ℓ ζ Hlabels Henabled.
-      rewrite Hex in Hlive. rewrite Heqn in Hlive. simpl.
-      assert (ℓ = Arole).
-      { rewrite /role_enabled_model in Henabled. simpl in *.
-        rewrite /retransmit_live_roles in Henabled. simpl in *.
-        set_solver. }
-      simplify_eq.
-      eapply from_locale_step; last first.
-      { eapply Hlive; [done|].
-        rewrite /role_enabled_model.
-        set_solver. }
-      eapply locale_step_atomic; eauto.
-      { f_equiv; [|done].
-        f_equiv. f_equiv. symmetry. apply app_nil_r. }
-      repeat econstructor; set_solver.
+      iApply wp_value'.
+      simpl.
+      rewrite !map_union_empty //.
+      do 4 wp_pure _.
+      iApply wp_value.
+      iApply "HΦ". iFrame. iSplit=>//.
+      iExists _, _, _. iFrame. iPureIntro; lia.
+  Qed.
+
+  Lemma wp_B tid f (Hf: f > 20):
+    {{{ inv Ns retinv ∗ own retransmit_name (◯E retransmit_model.Start) ∗
+          frag_free_roles_are ∅ ∗ is_node ipB ∗ saA ⤇ (λ _, True) ∗ saB ⤇ (λ _, True) ∗
+          (ipB, tid) ↦M {[ Brole := f ]} ∗ saB ⤳ (∅, ∅) ∗
+          free_ports (ip_of_address saB) {[port_of_address saB]} }}}
+      (mkExpr (ip_of_address saB) (Bprog saA saB)) @ (ipB, tid); ⊤
+    {{{ v, RET v; (ipB, tid) ↦M ∅ }}}.
+  Proof.
+    iIntros (Φ) "(#Hinv & Htok & #Hfr & #Hin & #HsockB & #HsockA & HB & Hrt & Hfp) HΦ".
+
+    rewrite /Bprog.
+    wp_bind (NewSocket _).
+
+    iApply sswp_MU_wp. iApply wp_new_socket=>//.
+    iIntros (sh) "Hsh'".
+
+    mu_fuel.
+    iApply wp_value'.
+
+    do 2 wp_pure _.
+
+    wp_bind (SocketBind _ _).
+    iApply sswp_MU_wp.
+    iApply (wp_socketbind with "[Hfp] [Hsh']")=>//=; first done.
+    iIntros "Hsh".
+    mu_fuel.
+    iApply wp_value'.
+    do 2 wp_pure _.
+
+    wp_bind (wait_receive _).
+
+    iApply (wp_wait _ _ with "[Hinv Hsh Hrt HB Htok]").
+    2: { iFrame "#∗". }
+    { lia. }
+    iNext.
+    iIntros (vv) "(%Heq & %f' & %R & %T & HB & %Hf' & Htok & Hrt & Hsh)".
+
+    do 2 wp_pure _.
+
+    iApply sswp_MU_wp_fupd.
+    iInv Ns as (st) "(Hst & Hrest)" "Hclose".
+    iModIntro.
+
+
+    iApply (wp_send _ _ false with "[Hsh] [Hrt] [HsockA]")=>//=>//=>//.
+    iNext. iIntros "Hsh HRT".
+
+    iDestruct (token_agree with "Hrest Htok") as %->.
+
+    iApply (mu_step_model _ _ _ _ ∅ ∅ _ (Done : lts_state retransmit_model) with "Hst [HB] [Hfr //]").
+    { constructor. }
+    { set_solver. }
+    { set_solver. }
+    { rewrite fmap_empty map_union_empty //. }
+    iIntros "Hst HB Hfr'".
+
+    iMod (token_update with "[Hrest Htok]") as "[Hrest Htok]".
+    { iFrame. }
+
+    iMod ("Hclose" with "[Hst Hrest]").
+    { iNext. iExists Done. iFrame. }
+    iModIntro.
+    simpl.
+
+    iApply wp_atomic.
+    { intros ????? Hs. apply val_stuck in Hs. done. }
+
+    iInv Ns as (st) "(Hst & Hrest)" "Hclose".
+    iModIntro.
+
+    iPoseProof (timeless with "Hst") as "Hst".
+    iPoseProof (timeless with "Hrest") as "Hrest".
+    iMod "Hst". iMod "Hrest".
+
+    iDestruct (token_agree with "Hrest Htok") as %->.
+
+    iMod (has_fuels_dealloc _ _ _ (Brole: usr_role retransmit_model) Done
+           with "Hst HB") as "[Hst HB]".
+    { set_solver. }
+
+    iApply wp_value'.
+
+    iMod ("Hclose" with "[Hst Hrest]").
+    { iNext. iExists Done. iFrame. }
+    iModIntro. iApply ("HΦ"). rewrite map_union_empty delete_insert //.
   Qed.
 
 End with_Σ.
