fairneris/aneris_lang/tactics.v
@@ -11,7 +11,6 @@ evaluation context [K] and a subexpression [e']. It calls the tactic [tac K e']
 for each possible decomposition until [tac] succeeds. *)
 Ltac reshape_expr e tac :=
   let rec go K e :=
-    idtac e;
     match e with
     | _                                 => tac K e
     | App ?e1 (Val ?v)                  => add_item (AppLCtx v) K e1
